dev/lf/paths/tight/Tight_possible_types.v
@@ -24,80 +24,75 @@ If S1 in SS and S2 in SS then (S1 & S2) in SS.
 If S in SS and G |-! y: {A: S..S} then y.A in SS.
  *)
 
-Inductive tight_pt : ctx -> var -> typ -> Prop :=
+Reserved Notation "G '|-##' p '::' T" (at level 40, p at level 59).
+
+Inductive tight_pt : ctx -> path -> typ -> Prop :=
   (* Precise typing *)
 | t_pt_precise : forall G x T,
-  ty_trm ty_precise sub_general G (trm_var (avar_f x)) T ->
-  tight_pt G x T
+    G |-! trm_path (p_var (avar_f x)) :: T ->
+    G |-## p_var (avar_f x) :: T
   (* Term member subtyping *)
-| t_pt_dec_trm : forall G x a T T',
-  tight_pt G x (typ_rcd (dec_trm a T)) ->
-  subtyp ty_general sub_tight G T T' ->
-  tight_pt G x (typ_rcd (dec_trm a T'))
+| t_pt_dec_trm : forall G p a m T T',
+    G |-## p :: typ_rcd (dec_trm a m T) ->
+    G |-# T <: T' ->
+    G |-## p :: typ_rcd (dec_trm a m T')
   (* Type member subtyping *)
-| t_pt_dec_typ : forall G x A T T' U' U,
-  tight_pt G x (typ_rcd (dec_typ A T U)) ->
-  subtyp ty_general sub_tight G T' T ->
-  subtyp ty_general sub_tight G U U' ->
-  tight_pt G x (typ_rcd (dec_typ A T' U'))
+| t_pt_dec_typ : forall G p A T T' U' U,
+    G |-## p :: typ_rcd (dec_typ A T U) ->
+    G |-# T' <: T ->
+    G |-# U <: U' ->
+    G |-## p :: typ_rcd (dec_typ A T' U')
   (* Recursive Types *)
-| t_pt_bnd : forall G x S S',
-  tight_pt G x S ->
-  S = open_typ x S' ->
-  tight_pt G x (typ_bnd S')
+| t_pt_bnd : forall G p S,
+    G |-## p :: open_typ_p p S ->
+    G |-## p :: typ_bnd S
   (* Forall *)
-| t_pt_all : forall L G x S T S' T',
-  tight_pt G x (typ_all S T) ->
-  subtyp ty_general sub_tight G S' S ->
-  (forall y, y \notin L ->
-   subtyp ty_general sub_general (G & y ~ S') (open_typ y T) (open_typ y T')) ->
-  tight_pt G x (typ_all S' T')
+| t_pt_all : forall L G p S T S' T',
+    G |-## p :: typ_all S T ->
+    G |-# S' <: S ->
+    (forall y, y \notin L ->
+      G & y ~ S' |- T ||^ y <: T' ||^ y) ->
+    G |-## p :: typ_all S' T'
   (* And *)
-| t_pt_and : forall G x S1 S2,
-  tight_pt G x S1 ->
-  tight_pt G x S2 ->
-  tight_pt G x (typ_and S1 S2)
+| t_pt_and : forall G p S1 S2,
+    G |-## p :: S1 ->
+    G |-## p :: S2 ->
+    G |-## p :: typ_and S1 S2
   (* Tight Selection *)
-| t_pt_sel : forall G x y A S,
-  tight_pt G x S ->
-  ty_trm ty_precise sub_general G (trm_var y) (typ_rcd (dec_typ A S S)) ->
-  tight_pt G x (typ_sel y A)
+| t_pt_sel : forall G p q A S,
+    G |-## p :: S ->
+    G |-! trm_path q :: typ_rcd (dec_typ A S S) ->
+    G |-## p :: typ_path q A
   (* Top *)
-| t_pt_top : forall G x T,
-  tight_pt G x T ->
-  tight_pt G x typ_top
-.
+| t_pt_top : forall G p T,
+    G |-## p :: T ->
+    G |-## p :: typ_top
+where "G '|-##' p '::' T" := (tight_pt G p T).
 
 Hint Constructors tight_pt.
 
-Lemma tight_possible_types_closure_tight: forall G x T U,
+Lemma tight_possible_types_closure_tight: forall G p T U,
   inert G ->
-  tight_pt G x T ->
-  subtyp ty_general sub_tight G T U ->
-  tight_pt G x U.
+  G |-## p :: T ->
+  G |-# T <: U ->
+  G |-## p :: U.
 Proof.
-  intros G x T U Hgd HT Hsub.
+  introv Hgd HT Hsub.
   dependent induction Hsub; eauto.
-  - inversion HT.
+  - inversion HT. inversions H1.
     destruct (inert_ty_precise_bot Hgd H).
-  - inversion HT.
-    + apply ty_precise_var_and_inv1 in H.
-      auto.
-    + auto.
-  - inversion HT.
-    + apply ty_precise_var_and_inv2 in H.
-      auto.
-    + auto.
-  - inversion HT.
+  - inversion* HT.
+  - inversion* HT.
+  - inversions HT.
     + false * inert_precise_sel_inv.
     + pose proof (inert_unique_tight_bounds Hgd H H5) as Hu. subst. assumption.
 Qed.
 
 Lemma tight_possible_types_lemma :
   forall G U x,
-    inert G -> (* G inert *)
-    ty_trm ty_general sub_tight G (trm_var (avar_f x)) U -> (* G |-# x : U *)
-    tight_pt G x U (* U \in TPT(G,x,T) *).
+    inert G ->
+    G |-# trm_var (avar_f x) :: U ->
+    G |-## x :: U.
 Proof.
   intros G U x Hgd Hty.
   dependent induction Hty.
